working on well-directioning

theories/DirectedDirectioning.v
@@ -3,64 +3,15 @@ From Coq Require Import ssreflect.
 From Equations Require Import Equations.
 From smpl Require Import Smpl.
 From LogRel.AutoSubst Require Import core unscoped Ast Extra.
-From LogRel Require Import Utils BasicAst Notations DirectedDirections DirectedContext GenericTyping.
+From LogRel Require Import Utils BasicAst Notations DirectedDirections Weakening Context.
 From Coq Require Import CRelationClasses.
 
 Set Primitive Projections.
 
-
-(* Import DeclarativeTypingData. *)
-(* Import DeclarativeTypingProperties. *)
-(* Import Notations. *)
-
 Reserved Notation "[ δ |- t ◃ d ]" (at level 0, δ, d, t at level 50, only parsing).
 Reserved Notation "[ δ |- t ▹ d ]" (at level 0, δ, d, t at level 50, only parsing).
 
-Notation "d1 ≦ d2" := (dir_leq d1 d2) (at level 70).
 
-Definition max_dir_opt d1 d2 : option direction :=
-  match d1, d2 with
-  | Discr, d => Some d
-  | Fun, Cofun => None
-  | Cofun, Fun => None
-  | d1, d2 => Some d1
-  end.
-
-Definition max_dir d1 d2 d3 := max_dir_opt d1 d2 = Some d3.
-
-Module MaxDirProp.
-Section MaxDirProp.
-
-  Lemma max_exists d1 d2 d : d1 ≦ d -> d2 ≦ d -> ∑ d', max_dir d1 d2 d'.
-  Proof.
-    destruct d, d1, d2; cbn; try easy.
-    all: intros _ _; eexists; unfold max_dir; cbn; reflexivity.
-  Qed.
-
-  Context (d1 d2 d3 : direction) (e : max_dir_opt d1 d2 = Some d3).
-
-  Lemma upper_bound1 : d1 ≦ d3.
-  Proof. 
-    destruct d1, d2, d3; cbn in *; try easy.
-    all: try injection e; discriminate.
-  Qed.
-
-  Lemma upper_bound2 : d2 ≦ d3.
-  Proof. 
-    destruct d1, d2, d3; cbn in *; try easy.
-    all: try injection e; discriminate.
-  Qed.
-
-  Lemma max_least d : d1 ≦ d -> d2 ≦ d -> d3 ≦ d.
-  Proof.
-    destruct d, d1, d2, d3; try easy + discriminate.
-  Qed.
-  
-End MaxDirProp.
-End MaxDirProp.
-
-
-(* TODO [TL]: note this is a "declarative" version, but we could also go algorithmic *)
 Inductive DirInfer (δ : list direction) : direction -> term -> Type :=
 | dirU : [ δ |- U ▹ Discr ]
 | dirVar {d n} :
@@ -83,6 +34,7 @@ with DirCheck (δ : list direction) : direction -> term -> Type :=
 where "[ δ |- t ▹ d ]" := (DirInfer δ d t)
 and "[ δ |- t ◃ d ]" := (DirCheck δ d t).
 
+(* TODO: use × instead of * *)
 Scheme DirInfer_mut_rect := Induction for DirInfer Sort Type with
     DirCheck_mut_rect := Induction for DirCheck Sort Type.
 
@@ -90,28 +42,63 @@ Combined Scheme DirInferCheck_rect from
   DirInfer_mut_rect,
   DirCheck_mut_rect.
 
+Definition dirU' {δ d} : [ δ |- U ◃ d ].
+Proof.
+  econstructor. 1: econstructor.
+  cbn; easy.
+Defined.
+
+Definition dirVar' {δ n d d'} :
+  List.nth_error δ n = Some d ->
+  d ⪯ d' -> [δ |- tRel n ◃ d'].
+Proof.
+  econstructor. 1: econstructor. all: tea.
+Defined.
+
+Definition dirProd' {δ d A B} :
+  [ δ |- A ◃ (dir_op d) ] -> [ cons Discr δ |- B ◃ d ] -> [ δ |- tProd A B ◃ d ].
+Proof.
+  intros hA hB. inversion hA; subst. inversion hB; subst.
+  assert (dir_op d0 ⪯ d) by (destruct d0, d; easy).
+  unshelve eassert (max := (MaxDirProp.max_exists (dir_op d0) d1 d _ _)); tea.
+  destruct max as [max ?].
+  econstructor. 1: econstructor.
+  1,2,3: tea.
+  eapply MaxDirProp.max_least; tea.
+Defined.
+
+Definition dirLam' {δ d A t} :
+  [ cons Discr δ |- t ◃ d ] ->
+  [ δ |- tLambda A t ◃ d ].
+Proof.
+  intros ht; inversion ht; subst.
+  econstructor. 1: econstructor.
+  all: tea.
+Defined.
+
+Definition dirApp' {δ d f a} :
+  [ δ |- f ◃ d ] ->
+  [ δ |- a ◃ Discr ] ->
+  [ δ |- tApp f a ◃ d ].
+Proof.
+  intros hf ha; inversion hf; subst.
+  econstructor. 1: econstructor.
+  all: tea.
+Defined.
+
 Definition dir_ren (ρ : nat -> nat) (δ γ : list direction) :=
-  forall n d, List.nth_error γ n = Some d -> 
+  forall n d, List.nth_error γ n = Some d ->
   ∑ d', (List.nth_error δ (ρ n) = Some d') × dir_leq d' d.
 
-Lemma dir_leq_trans d1 d2 d3 : dir_leq d1 d2 -> dir_leq d2 d3 -> dir_leq d1 d3.
-Proof.  destruct d1,d2, d3; easy. Qed.
 
-#[global]
-Instance: Transitive dir_leq := dir_leq_trans.
-
-
-Lemma dir_ren_up_discr {γ δ ρ} : dir_ren ρ δ γ -> dir_ren (up_ren ρ) (Discr :: δ) (Discr :: γ). 
+Lemma dir_ren_up_discr {γ δ ρ} : dir_ren ρ δ γ -> dir_ren (up_ren ρ) (Discr :: δ) (Discr :: γ).
 Proof.
   intros hρ [|n] d ; cbn.
   - intros [= <-]; exists Discr; now split.
   - intros [d' [-> ]]%hρ; exists d'; now split.
 Qed.
 
-Lemma dir_op_mon d1 d2 : d1 ≦ d2 -> dir_op d1 ≦ dir_op d2.
-Proof. destruct d1, d2; easy. Qed.
-
-Lemma dir_infer_check_ren γ 
+Lemma dir_infer_check_ren γ
   (Pinfer:= fun γ d t _ => forall δ ρ , dir_ren ρ δ γ -> ∑ d', [δ |- t⟨ρ⟩ ▹ d'] * dir_leq d' d)
   (Pcheck := fun γ d t _ => forall δ ρ , dir_ren ρ δ γ -> [δ |- t⟨ρ⟩ ◃ d])
 :
@@ -125,7 +112,7 @@ Proof.
     now etransitivity.
   }
   - econstructor; split; econstructor.
-  - intros * e * hρ. 
+  - intros * e * hρ.
     destruct (hρ _ _ e) as [? []].
     econstructor; split.
     1: now econstructor.
@@ -133,179 +120,96 @@ Proof.
   - intros * dirA ihA dirB ihB ? * hρ.
     destruct (ihA _ _ hρ) as [d1 [dirA' leq1]].
     destruct (ihB _ _ (dir_ren_up_discr hρ)) as [d2 [dirB' leq2]].
-    assert (dir_op d1 ≦ d''). 
+    assert (dir_op d1 ⪯ d'').
     by (etransitivity; try apply dir_op_mon; tea; now eapply MaxDirProp.upper_bound1).
-    assert (d2 ≦ d''). 
+    assert (d2 ⪯ d'').
     by (etransitivity; tea; now eapply MaxDirProp.upper_bound2).
     unshelve epose proof (MaxDirProp.max_exists (dir_op d1) d2 d'' _ _) as [d3]; tea.
     exists d3; split.
     1: now econstructor.
     eapply MaxDirProp.max_least; tea.
-  - admit.
-  - admit.
+  - intros * dirt iht ? * hρ.
+    destruct (iht _ _ (dir_ren_up_discr hρ)) as [d1 [dirt' leq1]].
+    eexists; split; tea.
+    now econstructor.
+  - intros * dirf ihf dira iha ? * hρ.
+    destruct (ihf _ _ hρ) as [d1 [dirf' leq1]].
+    eexists; split; tea.
+    constructor; tea.
+    now apply iha.
+Qed.
+
+Definition dir_subst {Γ Δ} (ρ : Γ ≤ Δ) (δ γ : list direction) :=
+  forall n d, List.nth_error γ n = Some d ->
+  ∑ d', (List.nth_error δ (ρ n) = Some d') × dir_leq d' d.
+
+Lemma dir_wk_up_discr {Γ Δ A γ δ} (ρ : Γ ≤ Δ) : dir_subst ρ δ γ -> dir_subst (wk_up A ρ) (Discr :: δ) (Discr :: γ).
+Proof.
+  intros hρ [|n] d ; cbn.
+  - intros [= <-]; exists Discr; now split.
+  - intros [d' [-> ]]%hρ; exists d'; now split.
+Qed.
+
+
+Lemma dir_infer_check_subst γ
+  (Pinfer:= fun γ d t _ => forall Γ Δ δ (ρ : Γ ≤ Δ) , dir_subst ρ δ γ -> ∑ d', [δ |- t⟨ρ⟩ ▹ d'] * dir_leq d' d)
+  (Pcheck := fun γ d t _ => forall Γ Δ δ (ρ : Γ ≤ Δ) , dir_subst ρ δ γ -> [δ |- t⟨ρ⟩ ◃ d])
+:
+  (forall d t (der : [γ |- t ▹ d]), Pinfer γ d t der)
+  * (forall d t (der : [γ |- t ◃ d]), Pcheck γ d t der).
+Proof.
+  apply DirInferCheck_rect.
+  all: unfold Pinfer, Pcheck.
+  6:{
+    intros * ? ih **; edestruct ih as [? []]; tea; econstructor; tea.
+    now etransitivity.
+  }
+  - econstructor; split; econstructor.
+  - intros * e * hρ.
+    destruct (hρ _ _ e) as [? []].
+    econstructor; split.
+    1: now econstructor.
+    tea.
+  - intros * dirA ihA dirB ihB ? * hρ.
+    destruct (ihA _ _ _ _ hρ) as [d1 [dirA' leq1]].
+    destruct (ihB _ _ _ _ (dir_wk_up_discr _ hρ (A:=A))) as [d2 [dirB' leq2]].
+    assert (dir_op d1 ⪯ d'').
+    by (etransitivity; try apply dir_op_mon; tea; now eapply MaxDirProp.upper_bound1).
+    assert (d2 ⪯ d'').
+    by (etransitivity; tea; now eapply MaxDirProp.upper_bound2).
+    unshelve epose proof (MaxDirProp.max_exists (dir_op d1) d2 d'' _ _) as [d3]; tea.
+    exists d3; split.
+    1: now econstructor.
+    eapply MaxDirProp.max_least; tea.
+  - intros * dirt iht ? * hρ.
+    destruct (iht _ _ _ _ (dir_wk_up_discr _ hρ (A:=A))) as [d1 [dirt' leq1]].
+    eexists; split; tea.
+    now econstructor.
+  - intros * dirf ihf dira iha ? * hρ.
+    destruct (ihf _ _ _ _ hρ) as [d1 [dirf' leq1]].
+    eexists; split; tea.
+    constructor; tea.
+    now apply iha.
+Qed.
+
+Lemma dir_subst_Discr {δ d B a} :
+  [ δ |- a ◃ Discr ] -> [ cons Discr δ |- B ◃ d ] -> [ δ |- B[a..] ◃ d ].
+Proof.
 Admitted.
 
+Inductive dir_ctx : context -> list direction -> list direction -> Type :=
+| dirNil : dir_ctx nil nil nil
+| dirCons {Γ δ δty A d dA} : DirCheck δ dA A -> dir_ctx (cons A Γ) (cons d δ) (cons dA δty).
 
-Inductive DirDecl : list direction -> direction -> term -> Type :=
-| dirU {δ d} : [ δ |- U @ d ]
-| dirVar {δ d d' n} :
-  List.nth_error δ n = Some d ->
-  dir_leq d d' ->
-  [ δ |- tRel n @ d' ]
-| dirProd {δ d A B} :
-  [ δ |- A @ dir_op d ] ->
-  [ cons Discr δ |- B @ d ] ->
-  [ δ |- tProd A B @ d ]
-| dirLam {δ d A t} :
-  [ cons Discr δ |- t @ d ] ->
-  [ δ |- tLambda A t @ d ]
-| dirApp {δ d f a} :
-  [ δ |- f @ d ] ->
-  [ δ |- a @ Discr ] ->
-  [ δ |- tApp f a @ d ]
-where "[ δ |- t @ d ]" := (DirDecl δ d t).
-
-
-
-(* TODO: check substitution lemmata for typing *)
-(* Lemma DirSubst {δ dB B da a} : *)
-(*   [ δ |- a @ da ] -> [ cons da δ |- B @ dB ] -> [ δ |- B[a..] @ dB ]. *)
-(* Proof. *)
-(*   intros wda wdB. *)
-(*   induction wdB. *)
-(*   - constructor. *)
-(*   - admit. *)
-(*   - cbn. *)
-
-
-Reserved Notation "[ |-( ) Γ ]" (at level 0, Γ at level 50, only parsing).
-Reserved Notation "[ Γ |-( d ) A ]" (at level 0, Γ, d, A at level 50, only parsing).
-Reserved Notation "[ Γ |-( dt ) t : A @( dA ) ]" (at level 0, Γ, dt, t, A, dA at level 50, only parsing).
-Reserved Notation "[ Γ |-( d ) A ≅ B ]" (at level 0, Γ, d, A, B at level 50, only parsing).
-Reserved Notation "[ Γ |-( dt ) t ≅ t' : A @( dA ) ]" (at level 0, Γ, dt, t, t', A, dA at level 50, only parsing).
-(* Reserved Notation "[ Γ |-( dt ) t ⤳* u ∈ A @( dA ) ]" (at level 0, Γ, dt, t, u, A, dA at level 50). *)
-
-Fixpoint WfCtx (ctx: context) : Type :=
-  match ctx with
-  | nil => unit
-  | cons {| ty := A ; ty_dir := dA ; dir := _ |} Θ =>
-      [ |-( ) Θ ] × [ List.map ty Θ |- A ] × [ List.map dir Θ |- A @ dA ]
-  end
-    where "[ |-( ) Θ ]" := (WfCtx Θ).
-
-
-Lemma WfCtx_erased {Θ: context} : [ |-( ) Θ ] -> [ |- List.map ty Θ ].
+Lemma dir_ctx_nth_ty {Γ δ δT n T dT} :
+  dir_ctx Γ δ δT ->
+  in_ctx Γ n T ->
+  List.nth_error δT n = Some dT ->
+  [δ |- T ◃ dT].
 Proof.
-  induction Θ.
-  - intros. constructor.
-  - intros [wfΘ [? ?]]. now constructor.
-Qed.
-
-Definition WfType (Θ: context) (d: direction) (A: term) : Type :=
-  [ |-( ) Θ ] × [ List.map ty Θ |- A ] × [ List.map dir Θ |- A @ d ].
-Notation "[ Θ |-( d ) A ]" := (WfType Θ d A).
-
-Lemma WfCtx_in_ctx {Θ d dA A} :
-  [ |-( ) Θ ] -> forall n, in_ctx Θ n {| ty := A; ty_dir := dA; dir := d |} ->
-  ([ List.map ty Θ |- A ] × [ List.map dir Θ |- A @ dA ]).
-Proof.
-Admitted.
-
-Lemma wfTypeU {Θ d} : [ |-( ) Θ ] -> [ Θ |-( d ) U ].
-Proof.
-  intros wfΘ.
-  constructor ; [ now trivial | split ].
-  - constructor. now eapply WfCtx_erased.
-  - constructor.
-Qed.
-
-Lemma wfTypeProd {Γ d} {A B} :
-  [ Γ |-( dir_op d ) A ] ->
-  [Γ ,, {| ty := A ; ty_dir := dir_op d ; dir := Discr |} |-( d ) B ] ->
-  [ Γ |-( d ) tProd A B ].
-Proof.
-  intros [wfA [? ?]] [wfB [? ?]].
-  constructor ; [ now trivial | split ].
-  all: now constructor.
-Qed.
-
-Definition Typing (Θ: context) (dt: direction) (T: term) (dT: direction) (t: term) :=
-  [ Θ |-( dT ) T ] × [ List.map ty Θ |- t : T ] × [ List.map dir Θ |- t @ dt ].
-Notation "[ Γ |-( dt ) t : T @( dT ) ]" := (Typing Γ dt T dT t).
-
-Lemma wfTypeUniv {Θ d} {A} :
-  [ Θ |-( d ) A : U @( Discr ) ] ->
-  [ Θ |-( d ) A ].
-Proof.
-  intros [[wfθ ?] [wtA wdA]].
-  constructor ; [ now trivial | split ].
-  - now apply wfTypeUniv.
-  - assumption.
-Qed.
-
-
-Lemma wfVar {Θ d'} {n d T dT} :
-  [ |-( ) Θ ] ->
-  in_ctx Θ n {| ty := T; ty_dir := dT; dir := d |} ->
-  dir_leq d d' ->
-  [ Θ |-( d' ) tRel n : T @( dT ) ].
-Proof.
-  intros wfΘ inΘ dleq.
-  split.
-  - constructor ; [ now trivial | split ].
-    + eapply WfCtx_in_ctx; tea.
-    + eapply WfCtx_in_ctx; tea.
-  - split.
-    + constructor.
-      * now apply WfCtx_erased.
-      * admit.
-    + eapply dirVar; tea.
-      clear wfΘ dleq d'.
-      revert Θ T dT d inΘ.
-      induction n.
-      * intros Θ T dT d inΘ. inversion inΘ; subst. reflexivity.
-      * intros Θ T dT d inΘ. inversion inΘ; subst; cbn.
-        now eapply IHn.
-Admitted.
-
-Lemma wfTermProd {Θ d} {A B} :
-  [ Θ |-( dir_op d ) A : U @( Discr ) ] ->
-  [ Θ ,, {| ty := A ; ty_dir := dir_op d ; dir := Discr |} |-( d ) B : U @( Discr ) ] ->
-  [ Θ |-( d ) tProd A B : U @( Discr ) ].
-Proof.
-  intros [[wfΘ ?] [wtA wdA]] [? [wtB wdB]].
-  split.
-  - constructor ; [ now trivial | split ].
-    all: now trivial.
-  - split.
-    1-2: now constructor.
-Qed.
-
-
-Lemma wfTermLam {Θ d} {dT A B t} :
-  [ Θ |-( dir_op dT ) A ] ->
-  [ Θ ,, {| ty := A ; ty_dir := dir_op dT ; dir := Discr |} |-( d ) t : B @( dT ) ] ->
-  [ Θ |-( d ) tLambda A t : tProd A B @( dT ) ].
-Proof.
-  intros [wfΘ [wtA wdA]] [[? [wtB wdB]] [wtt wdt]].
-  split.
-  - apply wfTypeProd. all: now constructor.
-  - split. all: now constructor.
-Qed.
-
-
-Lemma wfTermApp {Θ d} {dT f a A B} :
-  [ Θ |-( d ) f : tProd A B @( dT ) ] ->
-  [ Θ |-( Discr ) a : A @( dir_op dT ) ] ->
-  [ Θ |-( d ) tApp f a : B[a..] @( dT ) ].
-Proof.
-  intros [[wfΘ [wfProd wdProd]] [wtf wdf]] [[wfΘ' [wfA wdA]] [wta wda]].
-  split.
-  - constructor ; [ now trivial | split ].
-    + admit.
-    + (* will need substitution lemma *)
-      admit.
-  - split.
-    + now econstructor.
-    + now constructor.
+  intros dΓ inΓ.
+  induction inΓ.
+  - inversion dΓ; subst.
+    cbn.
+    admit.
 Admitted.
