theories/DirectedDirections.v
@@ -1,3 +1,6 @@
+From Coq Require Import ssreflect.
+From LogRel Require Import Utils.
+From Coq Require Import CRelationClasses.
 
 Inductive direction :=
 | Fun
@@ -23,3 +26,60 @@ Definition dir_leq (d1: direction) (d2: direction) : Type :=
   | Cofun, Fun => False
   end.
 
+
+Notation "d1 ⪯ d2" := (dir_leq d1 d2) (at level 70).
+
+Definition max_dir_opt d1 d2 : option direction :=
+  match d1, d2 with
+  | Discr, d => Some d
+  | Fun, Cofun => None
+  | Cofun, Fun => None
+  | d1, d2 => Some d1
+  end.
+
+Definition max_dir d1 d2 d3 := max_dir_opt d1 d2 = Some d3.
+
+Module MaxDirProp.
+Section MaxDirProp.
+
+  Lemma max_exists d1 d2 d : d1 ⪯ d -> d2 ⪯ d -> ∑ d', max_dir d1 d2 d'.
+  Proof.
+    destruct d, d1, d2; cbn; try easy.
+    all: intros _ _; eexists; unfold max_dir; cbn; reflexivity.
+  Qed.
+
+  Context (d1 d2 d3 : direction) (e : max_dir_opt d1 d2 = Some d3).
+
+  Lemma upper_bound1 : d1 ⪯ d3.
+  Proof. 
+    destruct d1, d2, d3; cbn in *; try easy.
+    all: try injection e; discriminate.
+  Qed.
+
+  Lemma upper_bound2 : d2 ⪯ d3.
+  Proof. 
+    destruct d1, d2, d3; cbn in *; try easy.
+    all: try injection e; discriminate.
+  Qed.
+
+  Lemma max_least d : d1 ⪯ d -> d2 ⪯ d -> d3 ⪯ d.
+  Proof.
+    destruct d, d1, d2, d3; try easy + discriminate.
+  Qed.
+  
+End MaxDirProp.
+End MaxDirProp.
+
+Lemma dir_leq_trans d1 d2 d3 : dir_leq d1 d2 -> dir_leq d2 d3 -> dir_leq d1 d3.
+Proof.  destruct d1,d2, d3; easy. Qed.
+
+#[global]
+Instance: Transitive dir_leq := dir_leq_trans.
+
+Lemma dir_leq_refl d : dir_leq d d.
+Proof. destruct d; easy. Qed.
+#[global]
+Instance: Reflexive dir_leq := dir_leq_refl.
+
+Lemma dir_op_mon d1 d2 : d1 ⪯ d2 -> dir_op d1 ⪯ dir_op d2.
+Proof. destruct d1, d2; easy. Qed.
