theories/DirectedTyping.v
@@ -1,0 +1,151 @@
+(** * LogRel.DeclarativeTyping: specification of conversion and typing, in a declarative fashion. *)
+From Coq Require Import ssreflect.
+From Equations Require Import Equations.
+From smpl Require Import Smpl.
+From LogRel.AutoSubst Require Import core unscoped Ast Extra.
+From LogRel Require Import Utils BasicAst Notations DirectedDirections DirectedContext DirectedDirectioning GenericTyping.
+
+Set Primitive Projections.
+
+Reserved Notation "[ |-( ) Γ ]" (at level 0, Γ at level 50, only parsing).
+Reserved Notation "[ Γ |-( d ) A ]" (at level 0, Γ, d, A at level 50, only parsing).
+Reserved Notation "[ Γ |-( dt ) t : A @( dA ) ]" (at level 0, Γ, dt, t, A, dA at level 50, only parsing).
+Reserved Notation "[ Γ |-( d ) A ≅ B ]" (at level 0, Γ, d, A, B at level 50, only parsing).
+Reserved Notation "[ Γ |-( dt ) t ≅ t' : A @( dA ) ]" (at level 0, Γ, dt, t, t', A, dA at level 50, only parsing).
+(* Reserved Notation "[ Γ |-( dt ) t ⤳* u ∈ A @( dA ) ]" (at level 0, Γ, dt, t, u, A, dA at level 50). *)
+
+
+Context `{ta : tag}
+  `{!WfContext ta} `{!WfType ta} `{!Typing ta}
+  `{!ConvType ta} `{!ConvTerm ta} `{!ConvNeuConv ta}
+  `{!RedType ta} `{!RedTerm ta}
+  `{!GenericTypingProperties ta _ _ _ _ _ _ _ _ _ _}.
+
+Record WfDirectedCtx (Θ: context) :=
+  { wf_ctx: [ |- List.map ty Θ ]
+  ; wf_ctx_dir: dir_ctx (List.map ty Θ) (List.map dir Θ) (List.map ty_dir Θ)
+  }.
+Notation "[ |-( ) Θ ]" := (WfDirectedCtx Θ).
+
+Record WfType (Θ: context) (d: direction) (A: term) :=
+  { wft: [ List.map ty Θ |- A ]
+  ; wft_ctx_dir: dir_ctx (List.map ty Θ) (List.map dir Θ) (List.map ty_dir Θ)
+  ; wft_dir: [ List.map dir Θ |- A ◃ d ]
+  }.
+Notation "[ Θ |-( d ) A ]" := (WfType Θ d A).
+
+(* TODO: note that I prove rules using naming convention from DeclarativeTyping *)
+Lemma wfTypeU {Θ d} : [ |-( ) Θ ] -> [ Θ |-( d ) U ].
+Proof.
+  intros [].
+  constructor; tea.
+  - now apply wft_U.
+  - now apply dirU'.
+Qed.
+
+Lemma wfTypeProd {Γ d} {A B} :
+  [ Γ |-( dir_op d ) A ] ->
+  [Γ ,, {| ty := A ; ty_dir := dir_op d ; dir := Discr |} |-( d ) B ] ->
+  [ Γ |-( d ) tProd A B ].
+Proof.
+  intros [] [].
+  constructor; tea.
+  - now apply wft_prod.
+  - now apply dirProd'.
+Qed.
+
+Record Typing (Θ: context) (dt: direction) (T: term) (dT: direction) (t: term) :=
+  { wt: [ List.map ty Θ |- t : T ]
+  ; wt_ctx_dir: dir_ctx (List.map ty Θ) (List.map dir Θ) (List.map ty_dir Θ)
+  ; wt_dir: [ List.map dir Θ |- t ◃ dt ]
+  ; wt_ty_dir: [ List.map dir Θ |- T ◃ dT ]
+  }.
+Notation "[ Γ |-( dt ) t : T @( dT ) ]" := (Typing Γ dt T dT t).
+
+Lemma wfTypeUniv {Θ d} {A} :
+  [ Θ |-( d ) A : U @( Discr ) ] ->
+  [ Θ |-( d ) A ].
+Proof.
+  intros [].
+  constructor; tea.
+  now apply wft_term.
+Qed.
+
+
+Lemma in_ctx_erased {Θ n decl} :
+  in_ctx Θ n decl -> Context.in_ctx (list_map ty Θ) n (ty decl).
+Proof.
+  induction 1; now constructor.
+Qed.
+
+Lemma in_ctx_nth_dir {Θ n decl} :
+  in_ctx Θ n decl -> List.nth_error (list_map dir Θ) n = Some (dir decl).
+Proof.
+  induction 1; tea.
+  reflexivity.
+Qed.
+
+Lemma in_ctx_nth_ty_dir {Θ n decl} :
+  in_ctx Θ n decl -> List.nth_error (list_map ty_dir Θ) n = Some (ty_dir decl).
+Proof.
+  induction 1; tea.
+  reflexivity.
+Qed.
+
+Lemma wfVar {Θ d'} {n d T dT} :
+  [ |-( ) Θ ] ->
+  in_ctx Θ n {| ty := T; ty_dir := dT; dir := d |} ->
+  dir_leq d d' ->
+  [ Θ |-( d' ) tRel n : T @( dT ) ].
+Proof.
+  intros [] inΘ leq.
+  split; tea.
+  - apply ty_var; tea.
+    now apply (in_ctx_erased (decl := {| ty := T; ty_dir := dT; dir := d |})).
+  - eapply dirVar'; tea.
+    now apply (in_ctx_nth_dir (decl := {| ty := T; ty_dir := dT; dir := d |})).
+  - eapply dir_ctx_nth_ty; tea.
+    + now apply (in_ctx_erased (decl := {| ty := T; ty_dir := dT; dir := d |})).
+    + now apply (in_ctx_nth_ty_dir (decl := {| ty := T; ty_dir := dT; dir := d |})).
+Qed.
+
+Lemma wfTermProd {Θ d} {A B} :
+  [ Θ |-( dir_op d ) A : U @( Discr ) ] ->
+  [ Θ ,, {| ty := A ; ty_dir := dir_op d ; dir := Discr |} |-( d ) B : U @( Discr ) ] ->
+  [ Θ |-( d ) tProd A B : U @( Discr ) ].
+Proof.
+  intros [] [].
+  split; tea.
+  - now apply ty_prod.
+  - now apply dirProd'.
+Qed.
+
+
+Lemma wfTermLam {Θ d} {dT A B t} :
+  [ Θ |-( dir_op dT ) A ] ->
+  [ Θ ,, {| ty := A ; ty_dir := dir_op dT ; dir := Discr |} |-( d ) t : B @( dT ) ] ->
+  [ Θ |-( d ) tLambda A t : tProd A B @( dT ) ].
+Proof.
+  intros [] [].
+  split; tea.
+  - now apply ty_lam.
+  - now apply dirLam'.
+  - now apply dirProd'.
+Qed.
+
+Lemma wfTermApp {Θ d} {dT f a A B} :
+  [ Θ |-( d ) f : tProd A B @( dT ) ] ->
+  [ Θ |-( Discr ) a : A @( dir_op dT ) ] ->
+  [ Θ |-( d ) tApp f a : B[a..] @( dT ) ].
+Proof.
+  intros [? ? ? wdProd] [].
+  split; tea.
+  - now eapply ty_app.
+  - now apply dirApp'.
+  - apply dir_subst_Discr; tea.
+    inversion wdProd; subst.
+    inversion X; subst.
+    econstructor; tea.
+    etransitivity; tea.
+    now eapply MaxDirProp.upper_bound2.
+Qed.
